riscv CRefine: complete proofs for ctz and clz
Signed-off-by: Mitchell Buckley <mitchell.buckley@data61.csiro.au>

proof/crefine/RISCV64/Machine_C.thy
@@ -132,12 +132,13 @@ lemma dmo_if:
 
 (* Count leading and trailing zeros. *)
 
-(* FIXME: move *)
+(* FIXME BV: move *)
 lemma word_ctz_max:
   "word_ctz w \<le> size w"
-  sorry
+  unfolding word_ctz_def
+  by (rule order_trans[OF List.length_takeWhile_le], clarsimp simp: word_size)
 
-(* FIXME move *)
+(* FIXME BV: move *)
 lemma scast_of_nat_small:
   "x < 2 ^ (LENGTH('a) - 1) \<Longrightarrow> scast (of_nat x :: 'a :: len word) = (of_nat x :: 'b :: len word)"
   apply (rule sym, subst word_unat.inverse_norm)
@@ -146,10 +147,10 @@ lemma scast_of_nat_small:
   apply (simp add: int_eq_sint unat_of_nat)
   done
 
-(* FIXME move *)
+(* FIXME BV: move *)
 lemmas casts_of_nat_small = ucast_of_nat_small scast_of_nat_small
 
-(* FIXME: move *)
+(* FIXME BV: move *)
 lemma hoarep_Seq_nothrow:
   assumes c: "hoarep \<Gamma> \<Theta> F P c Q {}"
   assumes d: "hoarep \<Gamma> \<Theta> F Q d R A"
@@ -162,15 +163,146 @@ definition clz32_step where
                  Guard ShiftError \<lbrace>\<acute>bits < SCAST(32 signed \<rightarrow> 32) 0x20\<rbrace> (\<acute>x___unsigned :== \<acute>x___unsigned >> unat \<acute>bits);;
                  \<acute>count :== \<acute>count - \<acute>bits"
 
-(* FIXME: figure out what this should be *)
 definition clz32_invariant where
-  "clz32_invariant i s \<equiv> {s'. undefined ''clz32_invariant'' i s s'}"
+  "clz32_invariant i s \<equiv> {s'.
+   mask___unsigned_' s' \<ge> x___unsigned_' s'
+   \<and> of_nat (word_clz (x___unsigned_' s')) + count_' s' = of_nat (word_clz (x___unsigned_' s)) + 32
+   \<and> mask___unsigned_' s' = mask (2 ^ unat i)}"
+
+\<comment>\<open> This function returns an expression stating that "if xs contains an element satisfying P, then
+    the nth element of xs is the *first* that satisfies P". \<close>
+definition first_in_list where
+  "first_in_list P n xs \<equiv> (\<forall>i. i < n \<longrightarrow> i < length xs \<longrightarrow> \<not> P (xs ! i)) \<and>
+                           (n < length xs \<longrightarrow> P (xs ! n))"
+
+\<comment>\<open> There is always some n at which P (x ! n) or P contains no such element \<close>
+lemma first_in_list_exists:
+  "\<exists>n. first_in_list P n xs"
+  apply (induction xs; simp add: first_in_list_def)
+  apply (erule exE)
+  apply (case_tac "P x1")
+   apply (rule_tac x=0 in exI, simp)
+  apply (rule_tac x="Suc n" in exI, clarsimp)
+  apply (case_tac i; simp)
+  done
+
+\<comment>\<open> If you know where P first fails to be true, then you know how to compute takeWhile with take. \<close>
+lemma takeWhile_take_equiv:
+  "first_in_list (not P) n xs \<Longrightarrow> takeWhile P xs = take n xs"
+  apply (rule takeWhile_eq_take_P_nth)
+  apply (clarsimp simp: first_in_list_def pred_neg_def)
+  apply (clarsimp simp: first_in_list_def pred_neg_def)
+  done
+
+\<comment>\<open> If you know that P fails to be true early enough, then truncating the input does not effect the
+    output of takeWhile. \<close>
+lemma takeWhile_truncate:
+  "length (takeWhile P xs) \<le> m
+  \<Longrightarrow> takeWhile P (take m xs) = takeWhile P xs"
+  apply (subgoal_tac "\<exists>n. first_in_list (not P) n xs")
+   apply (clarsimp)
+   apply (case_tac "n \<le> m")
+    apply (subgoal_tac "first_in_list (not P) n (take m xs)")
+     apply (drule takeWhile_take_equiv, simp)
+     apply (drule takeWhile_take_equiv, simp)
+    apply (clarsimp simp: first_in_list_def)
+   apply (subst (asm) takeWhile_take_equiv, assumption)
+   apply (clarsimp simp: first_in_list_def pred_neg_def)
+  apply (rule first_in_list_exists)
+  done
+
+lemma word_clz_shiftr_1:
+  fixes z::"'a::len word"
+  assumes wordsize: "1 < LENGTH('a)"
+  shows "z \<noteq> 0 \<Longrightarrow> word_clz (z >> 1) = word_clz z + 1"
+  supply word_size [simp]
+  apply (clarsimp simp: word_clz_def)
+  using wordsize apply (subst bl_shiftr, simp)
+  apply (subst takeWhile_append2; simp add: wordsize)
+  apply (subst takeWhile_truncate)
+  using word_clz_nonzero_max[where w=z]
+  apply (clarsimp simp: word_clz_def)
+  apply simp+
+  done
+
+(* FIXME BV: generalise and move *)
+lemma word_clz_1[simp]:
+  "word_clz (1::32 word) = 31"
+  "word_clz (1::64 word) = 63"
+  by (clarsimp simp: word_clz_def to_bl_def)+
+
+lemma shiftr_Suc:
+  fixes x::"'a::len word"
+  shows "x >> (Suc n) = x >> n >> 1"
+  by (clarsimp simp: shiftr_shiftr)
+
+lemma shiftl_Suc:
+  fixes x::"'a::len word"
+  shows "x << (Suc n) = x << n << 1"
+  by (clarsimp simp: shiftl_shiftl)
+
+lemma word_clz_shiftr:
+  fixes z::"'a::len word"
+  shows "n < LENGTH('a) \<Longrightarrow> z >> n \<noteq> 0 \<Longrightarrow> word_clz (z >> n) = word_clz z + n"
+  apply (induction n; simp)
+  apply (subgoal_tac "0 \<noteq> z >> n")
+  apply (subst shiftr_Suc)
+  apply (subst word_clz_shiftr_1; simp)
+  apply (clarsimp simp: word_less_nat_alt shiftr_div_2n' div_mult2_eq)
+  apply (case_tac "unat z div 2 ^ n = 0"; simp)
+  apply (clarsimp simp: div_eq_0_iff)
+  done
+
+lemma word_clz_shiftr':
+  fixes z::"'a::len word"
+  shows "n < LENGTH('a) \<Longrightarrow> z > mask n \<Longrightarrow> word_clz (z >> n) = word_clz z + n"
+  apply (erule word_clz_shiftr)
+  apply (clarsimp simp: mask_def)
+  apply (clarsimp simp: word_less_nat_alt word_le_nat_alt shiftr_div_2n' div_mult2_eq)
+  apply (case_tac "unat z div 2 ^ n = 0"; simp)
+  apply (clarsimp simp: div_eq_0_iff)
+  done
 
 lemma clz32_step:
-  "\<Gamma> \<turnstile> (clz32_invariant (i+1) s) clz32_step i (clz32_invariant i s)"
+  "unat (i :: 32 sword) < 5 \<Longrightarrow>
+   \<Gamma> \<turnstile> (clz32_invariant (i+1) s) clz32_step i (clz32_invariant i s)"
   unfolding clz32_step_def
   apply (vcg, clarsimp simp: clz32_invariant_def)
-  sorry
+  \<comment> \<open>Introduce some trivial but useful facts so that most later goals are solved with simp\<close>
+  apply (prop_tac "i \<noteq> -1", clarsimp simp: unat_minus_one_word)
+  apply (frule unat_Suc2)
+  apply (prop_tac "(2 :: nat) ^ unat i < (32 :: nat)",
+         clarsimp simp: power_strict_increasing_iff[where b=2 and y=5, simplified])
+  apply (prop_tac "(2 :: nat) ^ unat (i + 1) \<le> (32 :: nat)",
+         clarsimp simp: unat_Suc2 power_increasing_iff[where b=2 and y=4, simplified])
+  apply (intro conjI impI; clarsimp)
+       apply (clarsimp simp: word_less_nat_alt)
+      apply (erule le_shiftr)
+     apply (clarsimp simp: word_size shiftr_mask2 word_clz_shiftr')
+    apply (clarsimp simp: shiftr_mask2)
+   apply fastforce
+  apply (clarsimp simp: shiftr_mask2)
+  done
+
+(* FIXME BV: generalise this? *)
+lemma word32_le_1:
+  "(a :: 32 word) \<le> 1 = (a = 0 \<or> a = 1)"
+  apply (word_bitwise)
+  by fastforce
+
+lemma word64_le_1:
+  "(a :: 64 word) \<le> 1 = (a = 0 \<or> a = 1)"
+  apply (word_bitwise)
+  by fastforce
+
+(* FIXME BV: move *)
+lemma max_word_max32:
+  "(a :: 32 word) \<le> 0xFFFFFFFF"
+  by (word_bitwise)
+
+lemma max_word_max64:
+  "(a :: 64 word) \<le> 0xFFFFFFFFFFFFFFFF"
+  by (word_bitwise)
 
 lemma clz32_spec:
   "\<forall>s. \<Gamma> \<turnstile> {s} Call clz32_'proc \<lbrace>\<acute>ret__unsigned = of_nat (word_clz (x___unsigned_' s))\<rbrace>"
@@ -178,10 +310,10 @@ lemma clz32_spec:
   apply (hoarep_rewrite, fold clz32_step_def)
   apply (intro allI hoarep.Catch[OF _ hoarep.Skip])
   apply (rule_tac Q="clz32_invariant 0 s" in hoarep_Seq_nothrow[OF _ creturn_wp])
-  apply (rule HoarePartial.SeqSwap[OF clz32_step], simp)+
-  apply (rule conseqPre, vcg)
-  apply (all \<open>clarsimp simp: clz32_invariant_def\<close>)
-  sorry
+   apply (rule HoarePartial.SeqSwap[OF clz32_step], simp, simp)+
+   apply (rule conseqPre, vcg)
+   apply (all \<open>clarsimp simp: clz32_invariant_def mask_def max_word_max32\<close>)
+  by (fastforce simp: word32_le_1)
 
 definition clz64_step where
   "clz64_step i \<equiv> \<acute>mask___unsigned_longlong :== \<acute>mask___unsigned_longlong >> unat ((1::32 sword) << unat i);;
@@ -189,15 +321,39 @@ definition clz64_step where
                    Guard ShiftError \<lbrace>\<acute>bits < SCAST(32 signed \<rightarrow> 32) 0x40\<rbrace> (\<acute>x___unsigned_longlong :== \<acute>x___unsigned_longlong >> unat \<acute>bits);;
                    \<acute>count :== \<acute>count - \<acute>bits"
 
-(* FIXME: figure out what this should be *)
 definition clz64_invariant where
-  "clz64_invariant i s \<equiv> {s'. undefined ''clz64_invariant'' i s s'}"
+  "clz64_invariant i s \<equiv> {s'.
+   mask___unsigned_longlong_' s' \<ge> x___unsigned_longlong_' s'
+   \<and> of_nat (word_clz (x___unsigned_longlong_' s')) + count_' s' = of_nat (word_clz (x___unsigned_longlong_' s)) + 64
+   \<and> mask___unsigned_longlong_' s' = mask (2 ^ unat i)}"
 
 lemma clz64_step:
-  "\<Gamma> \<turnstile> (clz64_invariant (i+1) s) clz64_step i (clz64_invariant i s)"
+  "unat (i :: 32 sword) < 6 \<Longrightarrow>
+   \<Gamma> \<turnstile> (clz64_invariant (i+1) s) clz64_step i (clz64_invariant i s)"
   unfolding clz64_step_def
   apply (vcg, clarsimp simp: clz64_invariant_def)
-  sorry
+  \<comment> \<open>Introduce some trivial but useful facts so that most later goals are solved with simp\<close>
+  apply (prop_tac "i \<noteq> -1", clarsimp simp: unat_minus_one_word)
+  apply (frule unat_Suc2)
+  apply (prop_tac "(2 :: nat) ^ unat i < (64 :: nat)",
+         clarsimp simp: power_strict_increasing_iff[where b=2 and y=6, simplified])
+  apply (prop_tac "(2 :: nat) ^ unat (i + 1) \<le> (64 :: nat)",
+         clarsimp simp: unat_Suc2 power_increasing_iff[where b=2 and y=5, simplified])
+  apply (intro conjI impI; clarsimp)
+       apply (clarsimp simp: word_less_nat_alt)
+      apply (erule le_shiftr)
+     apply (clarsimp simp: word_size shiftr_mask2 word_clz_shiftr')
+    apply (clarsimp simp: shiftr_mask2)
+   apply fastforce
+  apply (clarsimp simp: shiftr_mask2)
+  done
+
+lemma word_clz_not_minus_1:
+  "of_nat (word_clz (w :: 64 word)) \<noteq> (max_word :: 32 word)"
+  unfolding not_max_word_iff_less
+  apply (rule word_of_nat_less)
+  apply (rule le_less_trans[OF word_clz_max[where w=w]])
+  by (simp add: word_size max_word_def)
 
 lemma clz64_spec:
   "\<forall>s. \<Gamma> \<turnstile> {s} Call clz64_'proc \<lbrace>\<acute>ret__unsigned = of_nat (word_clz (x___unsigned_longlong_' s))\<rbrace>"
@@ -205,10 +361,120 @@ lemma clz64_spec:
   apply (hoarep_rewrite, fold clz64_step_def)
   apply (intro allI hoarep.Catch[OF _ hoarep.Skip])
   apply (rule_tac Q="clz64_invariant 0 s" in hoarep_Seq_nothrow[OF _ creturn_wp])
-  apply (rule HoarePartial.SeqSwap[OF clz64_step], simp)+
-  apply (rule conseqPre, vcg)
-  apply (all \<open>clarsimp simp: clz64_invariant_def\<close>)
-  sorry
+   apply (rule HoarePartial.SeqSwap[OF clz64_step], simp, simp)+
+   apply (rule conseqPre, vcg)
+   apply (all \<open>clarsimp simp: clz64_invariant_def mask_def max_word_max64\<close>)
+  apply (clarsimp simp: word64_le_1)
+  apply (erule disjE; clarsimp)
+  apply (subst add.commute)
+  apply (subst ucast_increment[symmetric])
+   apply (rule word_clz_not_minus_1)
+  apply (clarsimp)
+  done
+
+lemma word_ctz_bound_below_helper:
+  fixes x :: "'a::len word"
+  assumes sz: "n \<le> LENGTH('a)"
+  shows "x && mask n = 0
+   \<Longrightarrow> to_bl x = (take (LENGTH('a) - n) (to_bl x) @ replicate n False)"
+  apply (subgoal_tac "replicate n False = drop (LENGTH('a) - n) (to_bl x)")
+   apply (subgoal_tac "True \<notin> set (drop (LENGTH('a) - n) (to_bl x))")
+    apply (drule list_of_false, clarsimp simp: sz)
+   apply (drule_tac sym[where t="drop n x" for n x], clarsimp)
+  apply (rule sym)
+  apply (rule is_aligned_drop; clarsimp simp: is_aligned_mask sz)
+  done
+
+lemma word_ctz_bound_below:
+  fixes x :: "'a::len word"
+  assumes sz[simp]: "n \<le> LENGTH('a)"
+  shows "x && mask n = 0 \<Longrightarrow> n \<le> word_ctz x"
+  apply (clarsimp simp: word_ctz_def)
+  apply (subst word_ctz_bound_below_helper[OF sz]; simp)
+  apply (subst takeWhile_append2; clarsimp)
+  done
+
+lemma mask_to_bl_exists_True:
+  "x && mask n \<noteq> 0 \<Longrightarrow> \<exists>m. (rev (to_bl x)) ! m \<and> m < n"
+  apply (subgoal_tac "\<not>(\<forall>m. m < n \<longrightarrow> \<not>(rev (to_bl x)) ! m)", fastforce)
+  apply (intro notI)
+  apply (subgoal_tac "x && mask n = 0", clarsimp)
+  apply (clarsimp simp: eq_zero_set_bl in_set_conv_nth)
+  apply (subst (asm) to_bl_nth, clarsimp simp: word_size)
+  apply (clarsimp simp: and_bang word_size)
+  apply (drule_tac x="LENGTH('a) - Suc i" in spec, simp)
+  apply (subst (asm) rev_nth, simp)
+  apply (subst (asm) to_bl_nth; clarsimp simp: word_size)
+  done
+
+lemma word_ctz_bound_above:
+  fixes x :: "'a::len word"
+  assumes sz: "n \<le> LENGTH('a)"
+  shows "x && mask n \<noteq> 0 \<Longrightarrow> word_ctz x < n"
+  apply (frule mask_to_bl_exists_True, clarsimp)
+  apply (clarsimp simp: word_ctz_def)
+  apply (subgoal_tac "m < length ((rev (to_bl x)))")
+  apply (subst id_take_nth_drop[where xs="rev (to_bl x)"], assumption)
+  apply (subst takeWhile_tail, simp)
+  apply (rule order.strict_trans1)
+  apply (rule List.length_takeWhile_le)
+  apply (simp add: length_take)
+  apply (erule order.strict_trans2, clarsimp simp: sz)
+  done
+
+lemma word_ctz_shiftr_1:
+  fixes z::"'a::len word"
+  assumes wordsize: "1 < LENGTH('a)"
+  shows "z \<noteq> 0 \<Longrightarrow> 1 \<le> word_ctz z \<Longrightarrow> word_ctz (z >> 1) = word_ctz z - 1"
+  supply word_size [simp]
+  apply (clarsimp simp: word_ctz_def)
+  using wordsize apply (subst bl_shiftr, simp)
+  apply (simp add: rev_take )
+   apply (subgoal_tac
+ "length (takeWhile Not (rev (to_bl z))) - Suc 0 = length (takeWhile Not (take 1 (rev (to_bl z)) @
+    drop 1 (rev (to_bl z)))) - Suc 0")
+   apply (subst (asm) takeWhile_append2)
+    apply clarsimp
+    apply (case_tac "rev (to_bl z)"; simp)
+   apply clarsimp
+   apply (subgoal_tac "\<exists>m. (rev (to_bl z)) ! m \<and> m < LENGTH('a)", clarsimp)
+    apply (case_tac m)
+     apply (case_tac "rev (to_bl z)"; simp)
+    apply (subst takeWhile_append1, subst in_set_conv_nth)
+      apply (rule_tac x=nat in exI)
+      apply (intro conjI)
+       apply (clarsimp simp: length_drop wordsize)
+       using wordsize
+       apply linarith
+      apply (rule refl, clarsimp)
+    apply simp
+   apply (rule mask_to_bl_exists_True, simp)
+  apply simp
+  done
+
+lemma word_ctz_shiftr:
+  fixes z::"'a::len word"
+  assumes nz: "z \<noteq> 0"
+  shows "n < LENGTH('a) \<Longrightarrow> n \<le> word_ctz z \<Longrightarrow> word_ctz (z >> n) = word_ctz z - n"
+  apply (induction n; simp)
+  apply (subst shiftr_Suc)
+  apply (subst word_ctz_shiftr_1, simp)
+    apply (clarsimp simp del: word_neq_0_conv)
+    apply (subgoal_tac "word_ctz z < n", clarsimp)
+    apply (rule word_ctz_bound_above, clarsimp simp: word_size)
+    apply (subst (asm) and_mask_eq_iff_shiftr_0[symmetric], clarsimp simp: nz)
+   apply (rule word_ctz_bound_below, clarsimp simp: word_size)
+   apply (rule mask_zero)
+   apply (rule is_aligned_shiftr, simp add: is_aligned_mask)
+   apply (case_tac "z && mask (Suc n) = 0", simp)
+   apply (frule word_ctz_bound_above[rotated]; clarsimp simp: word_size)
+   apply simp
+  done
+
+lemma word_ctz_0[simp]:
+  "word_ctz (0::32 word) = 32"
+  "word_ctz (0::64 word) = 64"
+  by (clarsimp simp: word_ctz_def to_bl_def)+
 
 definition ctz32_step where
   "ctz32_step i \<equiv> \<acute>mask___unsigned :== \<acute>mask___unsigned >> unat ((1::32 sword) << unat i);;
@@ -216,26 +482,79 @@ definition ctz32_step where
                    Guard ShiftError \<lbrace>\<acute>bits < SCAST(32 signed \<rightarrow> 32) 0x20\<rbrace> (\<acute>x___unsigned :== \<acute>x___unsigned >> unat \<acute>bits);;
                    \<acute>count :== \<acute>count + \<acute>bits"
 
-(* FIXME: figure out what this should be *)
 definition ctz32_invariant where
-  "ctz32_invariant i s \<equiv> {s'. undefined ''ctz32_invariant'' i s s'}"
+  "ctz32_invariant (i :: 32 sword) s \<equiv> {s'.
+     (x___unsigned_' s' \<noteq> 0 \<longrightarrow> (of_nat (word_ctz (x___unsigned_' s')) + count_' s' = of_nat (word_ctz (x___unsigned_' s))
+   \<and> (word_ctz (x___unsigned_' s') < 2 ^ unat i)))
+   \<and> (x___unsigned_' s' = 0 \<longrightarrow> (count_' s' + (0x1 << (unat i)) = 33 \<and> x___unsigned_' s = 0))
+   \<and> mask___unsigned_' s' = mask (2 ^ unat i)}"
+
+lemma mask_shiftr_zero:
+  "\<lbrakk>x && mask a = 0;  x >> a = 0\<rbrakk> \<Longrightarrow> x = 0"
+  by (simp add: and_mask_eq_iff_shiftr_0[symmetric])
+
+lemma word_ctz_32:
+  "word_ctz (x :: 32 word) = 32 \<Longrightarrow> x = 0"
+  apply (clarsimp simp: word_ctz_def)
+  apply (word_bitwise)
+  by (auto split: if_splits)
 
 lemma ctz32_step:
-  "\<Gamma> \<turnstile> (ctz32_invariant (i+1) s) ctz32_step i (ctz32_invariant i s)"
+  "unat (i :: 32 sword) < 5 \<Longrightarrow>
+   \<Gamma> \<turnstile> (ctz32_invariant (i+1) s) ctz32_step i (ctz32_invariant i s)"
+  supply word_neq_0_conv [simp del]
   unfolding ctz32_step_def
   apply (vcg, clarsimp simp: ctz32_invariant_def)
-  sorry
+  apply (prop_tac "i \<noteq> -1", clarsimp simp: unat_minus_one_word)
+  apply (frule unat_Suc2)
+  apply (prop_tac "(2 :: nat) ^ unat i < (32 :: nat)",
+         clarsimp simp: power_strict_increasing_iff[where b=2 and y=5, simplified])
+  apply (prop_tac "(2 :: nat) ^ unat (i + 1) \<le> (32 :: nat)",
+         clarsimp simp: unat_Suc2 power_increasing_iff[where b=2 and y=4, simplified])
+  apply (intro conjI; intro impI)
+   apply (intro conjI)
+      apply (clarsimp simp: word_less_nat_alt)
+     apply (intro impI)
+     apply (subgoal_tac "x___unsigned_' x \<noteq> 0")
+      apply (intro conjI, clarsimp)
+       apply (subst word_ctz_shiftr, clarsimp, clarsimp)
+        apply (rule word_ctz_bound_below, clarsimp simp: shiftr_mask2)
+        apply (clarsimp simp: shiftr_mask2 is_aligned_mask[symmetric])
+       apply (subst of_nat_diff)
+        apply (rule word_ctz_bound_below, clarsimp simp: shiftr_mask2)
+        apply (clarsimp simp: shiftr_mask2)
+     apply fastforce
+      apply (subst word_ctz_shiftr, clarsimp, clarsimp)
+       apply (rule word_ctz_bound_below, clarsimp simp: shiftr_mask2)
+       apply (clarsimp simp: shiftr_mask2 is_aligned_mask[symmetric])
+      apply (fastforce elim: is_aligned_weaken)
+     apply fastforce
+    apply (intro impI conjI; clarsimp simp: shiftr_mask2)
+     apply (subgoal_tac "x___unsigned_' x = 0", clarsimp)
+      apply (subst add.commute, simp)
+     apply (fastforce simp: shiftr_mask2 word_neq_0_conv elim: mask_shiftr_zero)
+    apply (frule (1) mask_shiftr_zero, simp)
+   apply (clarsimp simp: shiftr_mask2)
+  by (fastforce simp: shiftr_mask2 intro: word_ctz_bound_above)
 
 lemma ctz32_spec:
   "\<forall>s. \<Gamma> \<turnstile> {s} Call ctz32_'proc \<lbrace>\<acute>ret__unsigned = of_nat (word_ctz (x___unsigned_' s))\<rbrace>"
+  supply word_neq_0_conv [simp del]
   apply (hoare_rule HoarePartial.ProcNoRec1)
   apply (hoarep_rewrite, fold ctz32_step_def)
   apply (intro allI hoarep.Catch[OF _ hoarep.Skip])
   apply (rule_tac Q="ctz32_invariant 0 s" in hoarep_Seq_nothrow[OF _ creturn_wp])
-  apply (rule HoarePartial.SeqSwap[OF ctz32_step], simp)+
-  apply (rule conseqPre, vcg)
-  apply (all \<open>clarsimp simp: ctz32_invariant_def\<close>)
-  sorry
+   apply (rule HoarePartial.SeqSwap[OF ctz32_step], simp, simp)+
+   apply (rule conseqPre, vcg)
+   apply (clarsimp simp: ctz32_invariant_def)
+   apply (clarsimp simp: mask_def)
+   apply (subgoal_tac "word_ctz (x___unsigned_' s) \<le> size (x___unsigned_' s)")
+    apply (clarsimp simp: word_size)
+  using word_ctz_32 apply force
+   apply (rule word_ctz_max)
+  apply (clarsimp simp: ctz32_invariant_def)
+  apply (case_tac "x___unsigned_' x = 0"; clarsimp)
+  done
 
 definition ctz64_step where
   "ctz64_step i \<equiv> \<acute>mask___unsigned_longlong :== \<acute>mask___unsigned_longlong >> unat ((1::32 sword) << unat i);;
@@ -243,15 +562,61 @@ definition ctz64_step where
                    Guard ShiftError \<lbrace>\<acute>bits < SCAST(32 signed \<rightarrow> 32) 0x40\<rbrace> (\<acute>x___unsigned_longlong :== \<acute>x___unsigned_longlong >> unat \<acute>bits);;
                    \<acute>count :== \<acute>count + \<acute>bits"
 
-(* FIXME: figure out what this should be *)
 definition ctz64_invariant where
-  "ctz64_invariant i s \<equiv> {s'. undefined ''ctz64_invariant'' i s s'}"
+  "ctz64_invariant i s \<equiv> {s'.
+     (x___unsigned_longlong_' s' \<noteq> 0 \<longrightarrow> (of_nat (word_ctz (x___unsigned_longlong_' s')) + count_' s' = of_nat (word_ctz (x___unsigned_longlong_' s))
+   \<and> (word_ctz (x___unsigned_longlong_' s') < 2 ^ unat i)))
+   \<and> (x___unsigned_longlong_' s' = 0 \<longrightarrow> (count_' s' + (0x1 << (unat i)) = 65 \<and> x___unsigned_longlong_' s = 0))
+   \<and> mask___unsigned_longlong_' s' = mask (2 ^ unat i)}"
 
 lemma ctz64_step:
-  "\<Gamma> \<turnstile> (ctz64_invariant (i+1) s) ctz64_step i (ctz64_invariant i s)"
+  "unat (i :: 32 sword) < 6 \<Longrightarrow>
+   \<Gamma> \<turnstile> (ctz64_invariant (i+1) s) ctz64_step i (ctz64_invariant i s)"
+supply word_neq_0_conv [simp del]
   unfolding ctz64_step_def
   apply (vcg, clarsimp simp: ctz64_invariant_def)
-  sorry
+  apply (prop_tac "i \<noteq> -1", clarsimp simp: unat_minus_one_word)
+  apply (frule unat_Suc2)
+  apply (prop_tac "(2 :: nat) ^ unat i < (64 :: nat)",
+         clarsimp simp: power_strict_increasing_iff[where b=2 and y=6, simplified])
+  apply (prop_tac "(2 :: nat) ^ unat (i + 1) \<le> (64 :: nat)",
+         clarsimp simp: unat_Suc2 power_increasing_iff[where b=2 and y=5, simplified])
+  apply (intro conjI; intro impI)
+   apply (intro conjI)
+      apply (clarsimp simp: word_less_nat_alt)
+     apply (intro impI)
+     apply (subgoal_tac "x___unsigned_longlong_' x \<noteq> 0")
+      apply (intro conjI, clarsimp)
+       apply (subst word_ctz_shiftr, clarsimp, clarsimp)
+        apply (rule word_ctz_bound_below, clarsimp simp: shiftr_mask2)
+        apply (clarsimp simp: shiftr_mask2 is_aligned_mask[symmetric])
+       apply (subst of_nat_diff)
+        apply (rule word_ctz_bound_below, clarsimp simp: shiftr_mask2)
+        apply (clarsimp simp: shiftr_mask2)
+     apply fastforce
+      apply (subst word_ctz_shiftr, clarsimp, clarsimp)
+       apply (rule word_ctz_bound_below, clarsimp simp: shiftr_mask2)
+       apply (clarsimp simp: shiftr_mask2 is_aligned_mask[symmetric])
+      apply (fastforce elim: is_aligned_weaken)
+     apply fastforce
+    apply (intro impI conjI; clarsimp simp: shiftr_mask2)
+     apply (subgoal_tac "x___unsigned_longlong_' x = 0", clarsimp)
+      apply (subst add.commute, simp)
+     apply (fastforce simp: shiftr_mask2 word_neq_0_conv elim: mask_shiftr_zero)
+    apply (frule (1) mask_shiftr_zero, simp)
+   apply (clarsimp simp: shiftr_mask2)
+  by (fastforce simp: shiftr_mask2 intro: word_ctz_bound_above)
+
+lemma word_and_mask_word_ctz_zero:
+  assumes "l = word_ctz w"
+  shows "w && mask l = 0"
+  unfolding word_ctz_def assms
+  apply (word_eqI)
+  apply (drule takeWhile_take_has_property_nth)
+  apply (simp add: test_bit_bl)
+  done
+
+lemmas word_ctz_64 = word_and_mask_word_ctz_zero[where 'a=64 and l=64, simplified]
 
 lemma ctz64_spec:
   "\<forall>s. \<Gamma> \<turnstile> {s} Call ctz64_'proc \<lbrace>\<acute>ret__unsigned = of_nat (word_ctz (x___unsigned_longlong_' s))\<rbrace>"
@@ -259,10 +624,18 @@ lemma ctz64_spec:
   apply (hoarep_rewrite, fold ctz64_step_def)
   apply (intro allI hoarep.Catch[OF _ hoarep.Skip])
   apply (rule_tac Q="ctz64_invariant 0 s" in hoarep_Seq_nothrow[OF _ creturn_wp])
-  apply (rule HoarePartial.SeqSwap[OF ctz64_step], simp)+
-  apply (rule conseqPre, vcg)
-  apply (all \<open>clarsimp simp: ctz64_invariant_def\<close>)
-  sorry
+   apply (rule HoarePartial.SeqSwap[OF ctz64_step], simp, simp)+
+   apply (rule conseqPre, vcg)
+   apply (clarsimp simp: ctz64_invariant_def)
+   apply (clarsimp simp: mask_def)
+   apply (subgoal_tac "word_ctz (x___unsigned_longlong_' s) \<le> size (x___unsigned_longlong_' s)")
+    apply (clarsimp simp: word_size)
+    apply (erule le_neq_trans, clarsimp)
+  using word_ctz_64 apply force
+   apply (rule word_ctz_max)
+  apply (clarsimp simp: ctz64_invariant_def)
+  apply (case_tac "x___unsigned_longlong_' x = 0"; clarsimp)
+  done
 
 (* The library implementations would allow us to weaken the preconditions to allow zero inputs,
    but we keep the stronger preconditions to preserve older proofs that use these specs. *)
